chage(Predicate/FirstOrder/Basic/Term): Rew

Logic/Predicate/FirstOrder/Basic/Term/Term.lean
@@ -68,30 +68,28 @@ end Decidable
 
 abbrev func! (k) (f : L k) (v : Fin k → SubTerm L μ n) := func f v
 
-structure Hom (L : ℕ → Type u) (μ₁ : Type ν₁) (n₁ : ℕ) (μ₂ : Type ν₂) (n₂ : ℕ) where
+end SubTerm
+
+structure Rew (L : ℕ → Type u) (μ₁ : Type ν₁) (n₁ : ℕ) (μ₂ : Type ν₂) (n₂ : ℕ) where
   toFun : SubTerm L μ₁ n₁ → SubTerm L μ₂ n₂
-  func' : ∀ {k} (f : L k) (v : Fin k → SubTerm L μ₁ n₁), toFun (func f v) = func f (fun i => toFun (v i))
+  func' : ∀ {k} (f : L k) (v : Fin k → SubTerm L μ₁ n₁), toFun (SubTerm.func f v) = SubTerm.func f (fun i => toFun (v i))
 
-abbrev SyntacticHom (L : ℕ → Type u) (n₁ n₂ : ℕ) := Hom L ℕ n₁ ℕ n₂
+abbrev SyntacticRew (L : ℕ → Type u) (n₁ n₂ : ℕ) := Rew L ℕ n₁ ℕ n₂
 
-namespace Hom
+namespace Rew
 
-variable (ω : Hom L μ₁ n₁ μ₂ n₂)
+open SubTerm
+variable
+  {L L' : ℕ → Type u} {L₁ : ℕ → Type u₁} {L₂ : ℕ → Type u₂} {L₃ : ℕ → Type u₃}
+  {μ μ' : Type v} {μ₁ : Type v₁} {μ₂ : Type v₂} {μ₃ : Type v₃}
+  {n n₁ n₂ n₃ : ℕ}
+variable (ω : Rew L μ₁ n₁ μ₂ n₂)
 
-instance : FunLike (Hom L μ₁ n₁ μ₂ n₂) (SubTerm L μ₁ n₁) (fun _ => SubTerm L μ₂ n₂) where
+instance : FunLike (Rew L μ₁ n₁ μ₂ n₂) (SubTerm L μ₁ n₁) (fun _ => SubTerm L μ₂ n₂) where
   coe := fun f => f.toFun
   coe_injective' := fun f g h => by rcases f; rcases g; simp; exact h
 
-instance : CoeFun (Hom L μ₁ n₁ μ₂ n₂) (fun _ => SubTerm L μ₁ n₁ → SubTerm L μ₂ n₂) := ⟨Hom.toFun⟩
-
--- hide Hom.toFun
-open Lean PrettyPrinter Delaborator SubExpr in
-@[app_unexpander toFun]
-def unexpsnderToFun : Unexpander
-  | `($_ $h $x) => `($h $x)
-  | _           => throw ()
-
-@[ext] lemma ext (ω₁ ω₂ : Hom L μ₁ n₁ μ₂ n₂) (h : ∀ t, ω₁ t = ω₂ t) : ω₁ = ω₂ := FunLike.ext ω₁ ω₂ h
+instance : CoeFun (Rew L μ₁ n₁ μ₂ n₂) (fun _ => SubTerm L μ₁ n₁ → SubTerm L μ₂ n₂) := FunLike.hasCoeToFun
 
 protected lemma func {k} (f : L k) (v : Fin k → SubTerm L μ₁ n₁) :
     ω (func f v) = func f (fun i => ω (v i)) := ω.func' f v
@@ -100,49 +98,68 @@ lemma func'' {k} (f : L k) (v : Fin k → SubTerm L μ₁ n₁) :
     ω (func f v) = func f (ω ∘ v) := ω.func' f v
 
 @[simp] lemma func0 (f : L 0) (v : Fin 0 → SubTerm L μ₁ n₁) :
-    ω (func f v) = func f ![] := by simp[Hom.func]
+    ω (func f v) = func f ![] := by simp[Rew.func]
 
 @[simp] lemma func1 (f : L 1) (t : SubTerm L μ₁ n₁) :
-    ω (func f ![t]) = func f ![ω t] := by simp[Matrix.constant_eq_singleton, Hom.func]
+    ω (func f ![t]) = func f ![ω t] := by simp[Matrix.constant_eq_singleton, Rew.func]
 
 @[simp] lemma func2 (f : L 2) (t₁ t₂ : SubTerm L μ₁ n₁) :
-    ω (func f ![t₁, t₂]) = func f ![ω t₁, ω t₂] := by simp[Hom.func]; funext i; induction i using Fin.induction <;> simp
+    ω (func f ![t₁, t₂]) = func f ![ω t₁, ω t₂] := by simp[Rew.func]; funext i; induction i using Fin.induction <;> simp
 
 @[simp] lemma func3 (f : L 3) (t₁ t₂ t₃ : SubTerm L μ₁ n₁) :
     ω (func f ![t₁, t₂, t₃]) = func f ![ω t₁, ω t₂, ω t₃] := by
-  simp[Hom.func]; funext i; induction' i using Fin.induction with i <;> simp; induction' i using Fin.induction with i <;> simp 
+  simp[Rew.func]; funext i; induction' i using Fin.induction with i <;> simp; induction' i using Fin.induction with i <;> simp
 
-end Hom
+@[ext] lemma ext (ω₁ ω₂ : Rew L μ₁ n₁ μ₂ n₂) (hb : ∀ x, ω₁ #x = ω₂ #x) (hf : ∀ x, ω₁ &x = ω₂ &x) : ω₁ = ω₂ := by
+  apply FunLike.ext ω₁ ω₂; intro t
+  induction t <;> simp[*, ω₁.func, ω₂.func]
+
+lemma ext' {ω₁ ω₂ : Rew L μ₁ n₁ μ₂ n₂} (h : ω₁ = ω₂) (t) : ω₁ t = ω₂ t := by simp[h]
+
+protected def id : Rew L μ n μ n where
+  toFun := id
+  func' := fun _ _ => rfl
+
+@[simp] lemma id_app (t : SubTerm L μ n) : Rew.id t = t := rfl
+
+protected def comp (ω₂ : Rew L μ₂ n₂ μ₃ n₃) (ω₁ : Rew L μ₁ n₁ μ₂ n₂) : Rew L μ₁ n₁ μ₃ n₃ where
+  toFun := fun t => ω₂ (ω₁ t)
+  func' := fun f v => by simp[func'']; rfl
+
+lemma comp_app (ω₂ : Rew L μ₂ n₂ μ₃ n₃) (ω₁ : Rew L μ₁ n₁ μ₂ n₂) (t : SubTerm L μ₁ n₁) :
+    (ω₂.comp ω₁) t = ω₂ (ω₁ t) := rfl
 
 def bindAux (b : Fin n₁ → SubTerm L μ₂ n₂) (e : μ₁ → SubTerm L μ₂ n₂) : SubTerm L μ₁ n₁ → SubTerm L μ₂ n₂
   | (#x)       => b x    
   | (&x)       => e x
-  | (func f v) => func f (fun i => (v i).bindAux b e)
+  | (func f v) => func f (fun i => bindAux b e (v i))
 
-def bind (b : Fin n₁ → SubTerm L μ₂ n₂) (e : μ₁ → SubTerm L μ₂ n₂) : Hom L μ₁ n₁ μ₂ n₂ where
+def bind (b : Fin n₁ → SubTerm L μ₂ n₂) (e : μ₁ → SubTerm L μ₂ n₂) : Rew L μ₁ n₁ μ₂ n₂ where
   toFun := bindAux b e
   func' := fun _ _ => rfl
 
-abbrev rewrite (f : μ₁ → SubTerm L μ₂ n) : SubTerm L μ₁ n → SubTerm L μ₂ n := bind SubTerm.bvar f
+abbrev rewrite (f : μ₁ → SubTerm L μ₂ n) : Rew L μ₁ n μ₂ n := bind SubTerm.bvar f
 
-abbrev rewrite1 (t : SyntacticSubTerm L n) : SyntacticSubTerm L n → SyntacticSubTerm L n := bind SubTerm.bvar (t :>ₙ fvar)
-
-def map (b : Fin n₁ → Fin n₂) (e : μ₁ → μ₂) : Hom L μ₁ n₁ μ₂ n₂ :=
+def map (b : Fin n₁ → Fin n₂) (e : μ₁ → μ₂) : Rew L μ₁ n₁ μ₂ n₂ :=
   bind (fun n => #(b n)) (fun m => &(e m))
 
-def substs {n'} (v : Fin n → SubTerm L μ n') : Hom L μ n μ n' :=
+def substs {n'} (v : Fin n → SubTerm L μ n') : Rew L μ n μ n' :=
   bind v fvar
 
-scoped[FirstOrder] notation "ᵀ⟦→ " v "⟧" => SubTerm.substs v
-scoped[FirstOrder] notation "ᵀ⟦↦ " t "⟧" => SubTerm.substs ![t]
+def emb {o : Type v₁} [h : IsEmpty o] {μ : Type v₂} {n} : Rew L o n μ n := map id h.elim'
 
-def emb {o : Type w} [h : IsEmpty o] : Hom L o n μ n := map id h.elim'
-
-def bShift : Hom L μ n μ (n + 1) :=
+def bShift : Rew L μ n μ (n + 1) :=
   map Fin.succ id
 
-def castLe {n n' : ℕ} (h : n ≤ n') : Hom L μ n μ n' :=
+def castLe {n n' : ℕ} (h : n ≤ n') : Rew L μ n μ n' :=
   map (Fin.castLe h) id
+
+def q (ω : Rew L μ₁ n₁ μ₂ n₂) : Rew L μ₁ (n₁ + 1) μ₂ (n₂ + 1) := 
+  bind (#0 :> bShift ∘ ω ∘ bvar) (bShift ∘ ω ∘ fvar)
+
+lemma eq_id_of_eq {ω : Rew L μ n μ n} (hb : ∀ x, ω #x = #x) (he : ∀ x, ω &x = &x) (t) : ω t = t := by
+  have : ω = Rew.id := by ext <;> simp[*]
+  simp[this]
 
 section bind
 
@@ -152,36 +169,8 @@ variable (b : Fin n₁ → SubTerm L μ₂ n₂) (e : μ₁ → SubTerm L μ₂ 
 
 @[simp] lemma bind_bvar (n : Fin n₁) : bind b e (#n : SubTerm L μ₁ n₁) = b n := rfl
 
-@[simp] lemma bind_fbar' : bind b e ∘ fvar = e := by funext x; simp
-
-@[simp] lemma bind_bbar' : bind b e ∘ bvar = b := by funext x; simp
-
-lemma bind_bind
-  (b₁ : Fin n₁ → SubTerm L μ₂ n₂) (e₁ : μ₁ → SubTerm L μ₂ n₂)
-  (b₂ : Fin n₂ → SubTerm L μ₃ n₃) (e₂ : μ₂ → SubTerm L μ₃ n₃) (t : SubTerm L μ₁ n₁) :
-    bind b₂ e₂ (bind b₁ e₁ t) = bind (fun n => bind b₂ e₂ (b₁ n)) (fun m => bind b₂ e₂ (e₁ m)) t :=
-  by induction t <;> simp[*, Hom.func]
-
-lemma bind_bind'
-  (b₁ : Fin n₁ → SubTerm L μ₂ n₂) (e₁ : μ₁ → SubTerm L μ₂ n₂)
-  (b₂ : Fin n₂ → SubTerm L μ₃ n₃) (e₂ : μ₂ → SubTerm L μ₃ n₃) (t : SubTerm L μ₁ n₁) :
-    bind b₂ e₂ (bind b₁ e₁ t) = bind (bind b₂ e₂ ∘ b₁) (bind b₂ e₂ ∘ e₁) t :=
-  bind_bind _ _ _ _ _
-
-@[simp] lemma bind_id (t) : bind (L := L) (μ₁ := μ) (n₁ := n) bvar fvar t = t :=
-  by induction t <;> simp[*, Hom.func]
-
-@[simp] lemma bind_id_zero (f : Fin 0 → SubTerm L μ 0) (t) : bind (L := L) (μ₁ := μ) (n₁ := 0) f fvar t = t :=
-  by simpa[eq_finZeroElim] using bind_id t
-
-lemma bind_id_of_eq {b : Fin n → SubTerm L μ n} {e : μ → SubTerm L μ n}
-  (hb : ∀ x, b x = #x) (he : ∀ x, e x = &x) (t) : bind b e t = t := by
-  have e₁ : bvar = b := by funext x; simp[hb]
-  have e₂ : fvar = e := by funext x; simp[he]
-  exact e₁ ▸ e₂ ▸ bind_id t
-
-lemma Hom.eq_bind (ω : Hom L μ₁ n₁ μ₂ n₂) : ω = bind (ω ∘ bvar) (ω ∘ fvar) := by
-  ext t; induction t <;> simp[Hom.func'']; funext; simp[*]
+lemma eq_bind (ω : Rew L μ₁ n₁ μ₂ n₂) : ω = bind (ω ∘ bvar) (ω ∘ fvar) := by
+  ext t; induction t ; simp[Rew.func'']; funext; simp[*]
 
 end bind
 
@@ -193,25 +182,14 @@ variable (b : Fin n₁ → Fin n₂) (e : μ₁ → μ₂)
 
 @[simp] lemma map_bvar (n : Fin n₁) : map b e (#n : SubTerm L μ₁ n₁) = #(b n) := rfl
 
-@[simp] lemma map_fvar' : map (L := L) b e ∘ fvar = fvar ∘ e := rfl
-
-@[simp] lemma map_bvar' : map (L := L) b e ∘ bvar = bvar ∘ b := rfl
-
-lemma map_map
-  (b₁ : Fin n₁ → Fin n₂) (e₁ : μ₁ → μ₂)
-  (b₂ : Fin n₂ → Fin n₃) (e₂ : μ₂ → μ₃) (t : SubTerm L μ₁ n₁) :
-    map b₂ e₂ (map b₁ e₁ t) = map (b₂ ∘ b₁) (e₂ ∘ e₁) t :=
-  bind_bind _ _ _ _ _
-
-@[simp] lemma map_id (t) : @map L μ μ n n id id t = t :=
-  by induction t <;> simp[*, Hom.func]
+@[simp] lemma map_id : map (L := L) (id : Fin n → Fin n) (id : μ → μ) = Rew.id := by ext <;> simp
 
 lemma map_inj {b : Fin n₁ → Fin n₂} {e : μ₁ → μ₂} (hb : Function.Injective b) (he : Function.Injective e) :
     Function.Injective $ map (L := L) b e
-  | #x,                    t => by cases t <;> simp[Hom.func]; intro h; exact hb h
-  | &x,                    t => by cases t <;> simp[Hom.func]; intro h; exact he h
+  | #x,                    t => by cases t <;> simp[Rew.func]; intro h; exact hb h
+  | &x,                    t => by cases t <;> simp[Rew.func]; intro h; exact he h
   | func (arity := k) f v, t => by
-    cases t <;> simp[*, Hom.func]
+    cases t <;> simp[*, Rew.func]
     case func =>
       rintro rfl; simp; rintro rfl h; simp
       funext i; exact map_inj hb he (congr_fun h i)
@@ -220,7 +198,7 @@ end map
 
 section emb
 
-variable {o : Type w} [IsEmpty o]
+variable {o : Type v₂} [IsEmpty o]
 
 @[simp] lemma emb_bvar (x : Fin n) : emb (μ := μ) (#x : SubTerm L o n) = #x := rfl
 
@@ -231,9 +209,6 @@ section bShift
 @[simp] lemma bShift_bvar (x : Fin n) : bShift (#x : SubTerm L μ n) = #(Fin.succ x) := rfl
 
 @[simp] lemma bShift_fvar (x : μ) : bShift (&x : SubTerm L μ n) = &x := rfl
-
-lemma bShift_func {k} (f : L k) (v : Fin k → SubTerm L μ n) :
-  bShift (func f v) = func f (fun i => bShift (v i)) := rfl
 
 @[simp] lemma leftConcat_bShift_comp_bvar :
     (#0 :> bShift ∘ bvar : Fin (n + 1) → SubTerm L μ (n + 1)) = bvar :=
@@ -249,27 +224,63 @@ section substs
 
 variable {n'} (w : Fin n → SubTerm L μ n')
 
-@[simp] lemma substs_zero (w : Fin 0 → SubTerm L μ 0) (t : SubTerm L μ 0) : substs w t = t :=
-  by simp[substs]
-
 @[simp] lemma substs_bvar (x : Fin n) : substs w #x = w x :=
   by simp[substs]
 
 @[simp] lemma substs_fvar (x : μ) : substs w &x = &x :=
   by simp[substs]
 
-lemma substs_substs {l k} (v : Fin l → SubTerm L μ k) (w : Fin k → SubTerm L μ n) (t) :
-    substs w (substs v t) = substs (substs w ∘ v) t :=
-  by simp[substs, bind_bind, Function.comp]
+@[simp] lemma substs_zero (w : Fin 0 → Term L μ) : substs w = Rew.id :=
+  by ext x <;> simp; { exact Fin.elim0 x }
+
+lemma substs_comp_substs {l k} (v : Fin l → SubTerm L μ k) (w : Fin k → SubTerm L μ n) :
+    (substs w).comp (substs v) = substs (substs w ∘ v) :=
+  by ext <;> simp[comp_app]
 
 end substs
+
+section castLe
 
 @[simp] lemma castLe_bvar {n'} (h : n ≤ n') (x : Fin n) : castLe h (#x : SubTerm L μ n) = #(Fin.castLe h x) := rfl
 
 @[simp] lemma castLe_fvar {n'} (h : n ≤ n') (x : μ) : castLe h (&x : SubTerm L μ n) = &x := rfl
 
-lemma castLe_func {n'} (h : n ≤ n') {k} (f : L k) (v : Fin k → SubTerm L μ n) :
-    castLe h (func f v) = func f (fun i => castLe h (v i)) := rfl
+end castLe
+
+section q
+
+variable (ω : Rew L μ₁ n₁ μ₂ n₂)
+
+@[simp] lemma q_bvar_zero : ω.q #0 = #0 := by simp[Rew.q]
+
+@[simp] lemma q_bvar_succ (i : Fin n₁) : ω.q #(i.succ) = bShift (ω #i) := by simp[Rew.q]
+
+@[simp] lemma q_fvar (x : μ₁) : ω.q &x = bShift (ω &x) := by simp[Rew.q]
+
+@[simp] lemma q_comp_bShift : ω.q.comp bShift = bShift.comp ω := by
+  ext x <;> simp[comp_app]
+
+@[simp] lemma q_comp_bShift_app (t : SubTerm L μ₁ n₁) : ω.q (bShift t) = bShift (ω t) := by
+  have := ext' (ω.q_comp_bShift) t; simpa only [comp_app] using this
+
+@[simp] lemma q_id : (Rew.id : Rew L μ n μ n).q = Rew.id := by ext x; { cases x using Fin.cases <;> simp }; { simp }
+
+lemma q_comp (ω₂ : Rew L μ₂ n₂ μ₃ n₃) (ω₁ : Rew L μ₁ n₁ μ₂ n₂) :
+    (Rew.comp ω₂ ω₁).q = ω₂.q.comp ω₁.q := by ext x; { cases x using Fin.cases <;> simp[comp_app] }; { simp[comp_app] }
+
+lemma q_bind (b : Fin n₁ → SubTerm L μ₂ n₂) (e : μ₁ → SubTerm L μ₂ n₂) :
+    (bind b e).q = bind (#0 :> bShift ∘ b) (bShift ∘ e) := by ext x; { cases x using Fin.cases <;> simp }; { simp }
+
+lemma q_map (b : Fin n₁ → Fin n₂) (e : μ₁ → μ₂) :
+    (map (L := L) b e).q = map (0 :> Fin.succ ∘ b) e := by ext x; { cases x using Fin.cases <;> simp }; { simp }
+
+@[simp] lemma q_emb {o : Type v₁} [e : IsEmpty o] {n} :
+    (emb (L := L) (o := o) (μ := μ₂) (n := n)).q = emb := by ext x; { cases x using Fin.cases <;> simp }; { exact e.elim x }
+
+lemma q_substs (w : Fin n → SubTerm L μ n') :
+    (substs w).q = substs (#0 :> bShift ∘ w) := by ext x; { cases x using Fin.cases <;> simp }; { simp }
+
+end q
 
 section Syntactic
 
@@ -279,7 +290,7 @@ section Syntactic
   #0 #1 ... #(n - 1) &1 &2 &3 ...
 -/
 
-def shift : SyntacticHom L n n := map id Nat.succ
+def shift : SyntacticRew L n n := map id Nat.succ
 
 /- 
   #0 #1 ... #(n - 1) #n &0 &1 ...
@@ -287,9 +298,11 @@ def shift : SyntacticHom L n n := map id Nat.succ
   #0 #1 ... #(n - 1) &0 &1 &2 ...
  -/
 
-def free : SyntacticHom L (n + 1) n := bind (bvar <: &0) (fun m => &(Nat.succ m))
+def free : SyntacticRew L (n + 1) n := bind (bvar <: &0) (fun m => &(Nat.succ m))
 
-def fix : SyntacticHom L n (n + 1) := bind (fun x => #(Fin.castSucc x)) (#(Fin.last n) :>ₙ fvar)
+def fix : SyntacticRew L n (n + 1) := bind (fun x => #(Fin.castSucc x)) (#(Fin.last n) :>ₙ fvar)
+
+abbrev rewrite1 (t : SyntacticSubTerm L n) : SyntacticRew L n n := bind SubTerm.bvar (t :>ₙ fvar)
 
 section shift
 
@@ -302,13 +315,15 @@ lemma shift_func {k} (f : L k) (v : Fin k → SyntacticSubTerm L n) :
 
 lemma shift_Injective : Function.Injective (@shift L n) :=
   Function.LeftInverse.injective (g := map id Nat.pred)
-    (by intros p; simp[shift, map_map, Function.comp]; exact map_id _)
+    (by intros p; simp[←comp_app]; apply eq_id_of_eq <;> simp[comp_app])
 
 end shift
 
 section free
 
 @[simp] lemma free_bvar_castSucc (x : Fin n) : free (#(Fin.castSucc x) : SyntacticSubTerm L (n + 1)) = #x := by simp[free]
+
+@[simp] lemma free_bvar_castSucc_zero : free (#0 : SyntacticSubTerm L (n + 1 + 1)) = #0 := free_bvar_castSucc 0
 
 @[simp] lemma free_bvar_last : free (#(Fin.last n) : SyntacticSubTerm L (n + 1)) = &0 := by simp[free]
 
@@ -328,20 +343,81 @@ section fix
 
 end fix
 
-@[simp] lemma free_fix (t : SyntacticSubTerm L n) : free (fix t) = t :=
-  by simp[free, fix, bind_bind]; exact bind_id_of_eq (by simp) (by intro x; cases x <;> simp) t
+@[simp] lemma free_comp_fix : (free (L := L) (n := n)).comp fix = Rew.id := by
+  ext x <;> simp[comp_app]; { cases x <;> simp }
 
-@[simp] lemma fix_free (t : SyntacticSubTerm L (n + 1)) : fix (free t) = t :=
-  by simp[free, fix, bind_bind]; exact bind_id_of_eq (by intro x; cases x using Fin.lastCases <;> simp) (by simp) t
+@[simp] lemma fix_comp_free : (fix (L := L) (n := n)).comp free = Rew.id := by
+  ext x <;> simp[comp_app]; { cases x using Fin.lastCases <;> simp }
 
-@[simp] lemma bShift_free_eq_shift (t : SyntacticTerm L) : free (bShift t) = shift t :=
-  by simp[free, bShift, shift, map, bind_bind, eq_finZeroElim]
+@[simp] lemma bShift_free_eq_shift : (free (L := L) (n := 0)).comp bShift = shift := by
+  ext x <;> simp[comp_app]; { exact Fin.elim0 x }
 
-lemma substs_eq_substs1 (w : Fin (n + 1) → SyntacticTerm L) (t : SyntacticSubTerm L (n + 1)) :
-    substs w t = substs ![w $ Fin.last n] (fix $ substs (shift ∘ w ∘ Fin.castSucc) $ free t) :=
-  by simp[substs, free, fix, bind_bind]; congr; funext x; cases x using Fin.lastCases <;> simp[shift, map, bind_bind]
+lemma bShift_comp_substs (v : Fin n₁ → SubTerm L μ₂ n₂) :
+  bShift.comp (substs v) = substs (bShift ∘ v) := by ext x <;> simp[comp_app]
+
+lemma shift_comp_substs (v : Fin n₁ → SyntacticSubTerm L n₂) :
+  shift.comp (substs v) = (substs (shift ∘ v)).comp shift := by ext x <;> simp[comp_app]
+
+lemma shift_comp_substs1 (t : SyntacticSubTerm L n₂) :
+  shift.comp (substs ![t]) = (substs ![shift t]).comp shift := by ext x <;> simp[comp_app]
+
+@[simp] lemma rewrite_comp_emb {o : Type v₁} [e : IsEmpty o] (f : μ₂ → SubTerm L μ₃ n) :
+  (rewrite f).comp emb = (emb : Rew L o n μ₃ n) := by ext x <;> simp[comp_app]; { exact IsEmpty.elim e x }
+
+@[simp] lemma shift_comp_emb {o : Type v₁} [e : IsEmpty o] :
+  shift.comp emb = (emb : Rew L o n ℕ n) := by ext x <;> simp[comp_app]; { exact IsEmpty.elim e x }
+
+lemma rewrite_comp_free_eq_substs (t : SyntacticTerm L) :
+    (rewrite (t :>ₙ SubTerm.fvar)).comp free = substs ![t] := by ext x <;> simp[comp_app, Fin.eq_zero]
+
+lemma rewrite_comp_shift_eq_substs (t : SyntacticTerm L) :
+    (rewrite (t :>ₙ SubTerm.fvar)).comp shift = Rew.id := by ext x <;> simp[comp_app]
+
+lemma substs_mbar_zero_comp_shift_eq_free :
+    (substs (L := L) ![&0]).comp shift = free := by ext x <;> simp[comp_app, Fin.eq_zero]
+
+lemma free_comp_substs_eq_substs_comp_shift {n'} (w : Fin n' → SyntacticSubTerm Lf (n + 1)) :
+    free.comp (substs w) = (substs (free ∘ w)).comp shift :=
+  by ext x <;> simp[comp_app]
+
+section q
+
+variable (ω : SyntacticRew L n₁ n₂)
+
+@[simp] lemma q_shift : (shift (L := L) (n := n)).q = shift := by ext x; { cases x using Fin.cases <;> simp }; { simp }
+
+@[simp] lemma q_free : (free (L := L) (n := n)).q = free := by
+  ext x; { cases' x using Fin.cases with x <;> simp; { cases x using Fin.lastCases <;> simp[Fin.succ_castSucc] } }; { simp }
+
+@[simp] lemma q_fix : (fix (L := L) (n := n)).q = fix := by
+  ext x; { cases x using Fin.cases <;> simp[Fin.succ_castSucc] }; { cases x <;> simp }
+
+end q
 
 end Syntactic
+
+end Rew
+
+scoped syntax (name := substsNotation) "[→ " term,* "]" : term
+
+scoped macro_rules
+  | `([→ $terms:term,*]) => `(Rew.substs ![$terms,*])
+
+@[app_unexpander Rew.substs]
+def substsUnexpander : Lean.PrettyPrinter.Unexpander
+  | `($_ ![$terms,*]) => `([→ $terms,*])
+  | _ => throw ()
+
+scoped notation "⇑" => Rew.shift
+
+namespace SubTerm
+
+open Rew
+
+variable
+  {L L' : ℕ → Type u} {L₁ : ℕ → Type u₁} {L₂ : ℕ → Type u₂}
+  {μ μ' : Type v} {μ₁ : Type v₁} {μ₂ : Type v₂} {μ₃ : Type v₃}
+  {n n₁ n₂ n₃ : ℕ}
 
 def fvarList : SubTerm L μ n → List μ
   | #_       => []
@@ -361,7 +437,7 @@ abbrev fvar? (t : SubTerm L μ n) (x : μ) : Prop := x ∈ t.fvarList
 lemma bind_eq_of_funEqOn (b : Fin n₁ → SubTerm L μ₂ n₂) (e₁ e₂ : μ₁ → SubTerm L μ₂ n₂) (t : SubTerm L μ₁ n₁)
   (h : Function.funEqOn t.fvar? e₁ e₂) :
     bind b e₁ t = bind b e₂ t := by
-  induction t <;> simp[Hom.func]
+  induction t <;> simp[Rew.func]
   case fvar => simpa[fvar?, Function.funEqOn] using h
   case func k f v ih =>
     funext i
@@ -403,7 +479,7 @@ lemma lMap_func {k} (f : L₁ k) (v : Fin k → SubTerm L₁ μ n) :
 
 lemma lMap_bind (b : Fin n₁ → SubTerm L₁ μ₂ n₂) (e : μ₁ → SubTerm L₁ μ₂ n₂) (t) :
     (bind b e t).lMap Φ = bind (fun x => (b x).lMap Φ) (fun x => (e x).lMap Φ) (t.lMap Φ) :=
-  by induction t <;> simp[*, lMap_func, Hom.func]
+  by induction t <;> simp[*, lMap_func, Rew.func]
 
 lemma lMap_map (b : Fin n₁ → Fin n₂) (e : μ₁ → μ₂) (t) :
     (map b e t).lMap Φ = map b e (t.lMap Φ) :=
@@ -425,8 +501,8 @@ end lMap
 
 structure Operator (L : ℕ → Type u) (ι : Type w) where
   operator : {μ : Type v} → {n : ℕ} → (ι → SubTerm L μ n) → SubTerm L μ n
-  bind_operator : ∀ {μ μ' n₁ n₂} (b : Fin n₁ → SubTerm L μ' n₂) (e : μ → SubTerm L μ' n₂) (v : ι → SubTerm L μ n₁),
-    bind b e (operator v) = operator (fun i => bind b e (v i))
+  rew_operator : ∀ {μ μ' n₁ n₂} (ω : Rew L μ n₁ μ' n₂) (v : ι → SubTerm L μ n₁),
+    ω (operator v) = operator (fun i => ω (v i))
 
 abbrev Const (L : ℕ → Type u) := Operator.{u,v,0} L Empty
 
@@ -434,46 +510,9 @@ abbrev Monadic (L : ℕ → Type u) := Operator L Unit
 
 abbrev Finitary (L : ℕ → Type u) (n : ℕ) := Operator L (Fin n)
 
-namespace Operator
+def Operator.const (c : Const L) : SubTerm L μ n := c.operator Empty.elim
 
-variable {ι : Type w}
-
-def const (c : Const L) : SubTerm L μ n := c.operator Empty.elim
-
-instance : Coe (Const L) (SubTerm L μ n) := ⟨const⟩
-
-lemma bind_const (b : Fin n₁ → SubTerm L μ' n₂) (e : μ → SubTerm L μ' n₂) (c : Const L) :
-    bind b e c = c :=
-  by simpa[const, Empty.eq_elim] using c.bind_operator b e Empty.elim
-
-end Operator
-
-namespace Hom
-
-variable (ω : Hom L μ n₁ μ' n₂)
-
-protected lemma operator (o : Operator L ι) (v : ι → SubTerm L μ n₁) :
-    ω (o.operator v) = o.operator (fun i => ω (v i)) := by rw[ω.eq_bind]; exact o.bind_operator _ _ _
-
-protected lemma operator' (o : Operator L ι) (v : ι → SubTerm L μ n₁) :
-    ω (o.operator v) = o.operator (ω ∘ v) := ω.operator o v
-
-@[simp] lemma finitary0 (o : Finitary L 0) (v : Fin 0 → SubTerm L μ n₁) :
-    ω (o.operator v) = o.operator ![] := by simp[ω.operator', Matrix.empty_eq]
-
-@[simp] lemma finitary1 (o : Finitary L 1) (t : SubTerm L μ n₁) :
-    ω (o.operator ![t]) = o.operator ![ω t] := by simp[ω.operator']
-
-@[simp] lemma finitary2 (o : Finitary L 2) (t₁ t₂ : SubTerm L μ n₁) :
-    ω (o.operator ![t₁, t₂]) = o.operator ![ω t₁, ω t₂] := by simp[ω.operator']
-
-@[simp] lemma finitary3 (o : Finitary L 3) (t₁ t₂ t₃ : SubTerm L μ n₁) :
-    ω (o.operator ![t₁, t₂, t₃]) = o.operator ![ω t₁, ω t₂, ω t₃] := by simp[ω.operator']
-
-@[simp] protected lemma const (c : Const L) :
-    ω c = c := by rw[ω.eq_bind]; exact Operator.bind_const _ _ _
-
-end Hom
+instance : Coe (Const L) (SubTerm L μ n) := ⟨Operator.const⟩
 
 section natLit
 
@@ -491,7 +530,7 @@ def addOnes (t : SubTerm L μ n) : ℕ → SubTerm L μ n
 @[simp] lemma addOnes_succ (t : SubTerm L μ n) (z : ℕ) :
   addOnes t (z + 1) = func Language.Add.add ![addOnes t z, func Language.One.one ![]] := rfl
 
-lemma Hom.addOnes (ω : Hom L μ₁ n₁ μ₂ n₂) (t : SubTerm L μ₁ n₁) (z : ℕ) :
+lemma Rew.addOnes (ω : Rew L μ₁ n₁ μ₂ n₂) (t : SubTerm L μ₁ n₁) (z : ℕ) :
     ω (t.addOnes z) = (ω t).addOnes z := by induction z <;> simp[*]
 
 -- (((((1 + 1) + 1) + 1) + 1) ... ) 
@@ -503,7 +542,7 @@ variable (L)
 
 def natLit (z : ℕ) : Const L where
   operator := fun _ => natLit' z
-  bind_operator := by intros; cases z <;> simp[natLit', Hom.addOnes, Matrix.empty_eq]
+  rew_operator := by intros; cases z <;> simp[natLit', Rew.addOnes, Matrix.empty_eq]
 
 variable {L}
 
@@ -522,5 +561,38 @@ lemma natLit_succ (z : ℕ) (neZero : z ≠ 0) :
 end natLit
 
 end SubTerm
+
+namespace Rew
+
+open SubTerm
+
+variable
+  {L L' : ℕ → Type u} {L₁ : ℕ → Type u₁} {L₂ : ℕ → Type u₂}
+  {μ μ' : Type v} {μ₁ : Type v₁} {μ₂ : Type v₂} {μ₃ : Type v₃}
+  {n n₁ n₂ n₃ : ℕ}
+variable (ω : Rew L μ n₁ μ' n₂)
+
+protected lemma operator (o : Operator L ι) (v : ι → SubTerm L μ n₁) :
+    ω (o.operator v) = o.operator (fun i => ω (v i)) := by rw[ω.eq_bind]; exact o.rew_operator _ _
+
+protected lemma operator' (o : Operator L ι) (v : ι → SubTerm L μ n₁) :
+    ω (o.operator v) = o.operator (ω ∘ v) := ω.operator o v
+
+@[simp] lemma finitary0 (o : Finitary L 0) (v : Fin 0 → SubTerm L μ n₁) :
+    ω (o.operator v) = o.operator ![] := by simp[ω.operator', Matrix.empty_eq]
+
+@[simp] lemma finitary1 (o : Finitary L 1) (t : SubTerm L μ n₁) :
+    ω (o.operator ![t]) = o.operator ![ω t] := by simp[ω.operator']
+
+@[simp] lemma finitary2 (o : Finitary L 2) (t₁ t₂ : SubTerm L μ n₁) :
+    ω (o.operator ![t₁, t₂]) = o.operator ![ω t₁, ω t₂] := by simp[ω.operator']
+
+@[simp] lemma finitary3 (o : Finitary L 3) (t₁ t₂ t₃ : SubTerm L μ n₁) :
+    ω (o.operator ![t₁, t₂, t₃]) = o.operator ![ω t₁, ω t₂, ω t₃] := by simp[ω.operator']
+
+@[simp] protected lemma const (c : Const L) : ω c = c :=
+  by simpa[Operator.const, Empty.eq_elim] using c.rew_operator ω Empty.elim
+
+end Rew
 
 end FirstOrder
