Logic/Predicate/FirstOrder/Basic/Term/Elab.lean
@@ -1,4 +1,4 @@
-import Logic.Predicate.Term
+import Logic.Predicate.FirstOrder.Basic.Term.Term
 
 namespace FirstOrder
 
@@ -9,7 +9,7 @@ syntax:max "#" term:max : subterm
 syntax:max "&" term:max : subterm
 syntax:max "ᵀ!" term:max : subterm
 syntax num : subterm
-syntax:70 "[" term "](" subterm,* ")" : subterm
+syntax:70 "ᵀ⟨" term "⟩(" subterm,* ")" : subterm
 syntax:50 subterm:50 " + " subterm:51 : subterm
 syntax:60 subterm:60 " * " subterm:61 : subterm
 syntax:65 subterm:65 " ^ " subterm:66 : subterm
@@ -18,22 +18,20 @@ syntax:75 "⟨" subterm ", " subterm "⟩" : subterm
 
 syntax "(" subterm ")" : subterm
 
-syntax subterm "ᵀ⟦" subterm,* "⟧" : subterm
+syntax subterm "ᵀ[" subterm,* "]" : subterm
 syntax:80 "⤒" subterm:80 : subterm
 syntax:80 "ᵀ⇑" subterm:80 : subterm
 syntax:80 "ᵀᶠ" subterm:80 : subterm
 syntax:80 "ᵀᵇ" subterm:80 : subterm
 
 syntax "ᵀ“" subterm:0 "”" : term
-
-#check SubTerm.fix
  
 macro_rules
   | `(ᵀ“ # $n:term”)                                 => `(#$n)
   | `(ᵀ“ & $n:term ”)                                => `(&$n)
   | `(ᵀ“ ᵀ! $t:term ”)                               => `($t)
   | `(ᵀ“ $n:num ”)                                   => `(SubTerm.Operator.const (natLit _ $n))
-  | `(ᵀ“ [ $d:term ]( $t:subterm,* ) ”)              => do
+  | `(ᵀ“ ᵀ⟨ $d:term ⟩( $t:subterm,* ) ”)              => do
     let v ← t.getElems.foldrM (β := Lean.TSyntax _) (init := ← `(![])) (fun a s => `(ᵀ“$a” :> $s))
     `(func $d $v)
   | `(ᵀ“ $t:subterm + $u:subterm ”)                  => `(func Language.Add.add ![ᵀ“$t”, ᵀ“$u”])
@@ -41,19 +39,19 @@ macro_rules
   | `(ᵀ“ $t:subterm ^ $u:subterm ”)                  => `(func Language.Pow.pow ![ᵀ“$t”, ᵀ“$u”])
   | `(ᵀ“ exp $t:subterm ”)                           => `(func Language.Exp.exp ![ᵀ“$t”])
   | `(ᵀ“ ⟨ $t:subterm, $u:subterm ⟩ ”)               => `(func Language.Pairing.pair ![ᵀ“$t”, ᵀ“$u”])
-  | `(ᵀ“ ᵀ⇑$t:subterm ”)                            => `(shift ᵀ“$t”)
-  | `(ᵀ“ $t:subterm ᵀ⟦$u:subterm,*⟧ ”)               => do
+  | `(ᵀ“ ᵀ⇑$t:subterm ”)                            => `(Rew.shift ᵀ“$t”)
+  | `(ᵀ“ $t:subterm ᵀ[$u:subterm,*] ”)               => do
     let v ← u.getElems.foldrM (β := Lean.TSyntax _) (init := ← `(![])) (fun a s => `(ᵀ“$a” :> $s))
-    `(substs $v ᵀ“$t”)
-  | `(ᵀ“ ⤒$t:subterm ”)                             => `(SubTerm.bShift ᵀ“$t”)
-  | `(ᵀ“ ᵀᶠ $t:subterm ”)                            => `(SubTerm.free ᵀ“$t”)
-  | `(ᵀ“ ᵀᵇ $t:subterm ”)                            => `(SubTerm.fix ᵀ“$t”)
+    `(Rew.substs $v ᵀ“$t”)
+  | `(ᵀ“ ⤒$t:subterm ”)                             => `(Rew.bShift ᵀ“$t”)
+  | `(ᵀ“ ᵀᶠ $t:subterm ”)                            => `(Rew.free ᵀ“$t”)
+  | `(ᵀ“ ᵀᵇ $t:subterm ”)                            => `(Rew.fix ᵀ“$t”)
   | `(ᵀ“ ( $x ) ”)                                   => `(ᵀ“$x”)
 
 #check Language.Add.add
 
-#check (ᵀ“ [Language.ORingFunc.mul](&2 + &0, [Language.ORingFunc.zero]())” : SubTerm Language.ORingFunc ℕ 8)
-#check (ᵀ“ [Language.ORingFunc.mul](&2 + &0, [Language.ORingFunc.zero]())” : SubTerm Language.ORingFunc ℕ 8)
+#check (ᵀ“ ᵀ⟨Language.ORingFunc.mul⟩(&2 + &0, ᵀ⟨Language.ORingFunc.zero⟩())” : SubTerm Language.ORingFunc ℕ 8)
+#check (ᵀ“ ᵀ⟨Language.ORingFunc.mul⟩(&2 + &0, ᵀ⟨Language.ORingFunc.zero⟩())” : SubTerm Language.ORingFunc ℕ 8)
 #check ᵀ“ᵀ⇑(3 * #3 + 9)”
 #check SubTerm.func Language.Mul.mul (ᵀ“1” :> ᵀ“3” :> Matrix.vecEmpty)
 
@@ -79,7 +77,7 @@ notation "lang(^)" => Language.Pow.pow
 notation "lang(exp)" => Language.Exp.exp
 notation "lang(⟨⟩)" => Language.Pairing.pair
 
-@[app_unexpander Language.Add.add]
+@[app_unexpander Language.Add.add] 
 def unexpsnderAdd : Unexpander
   | `($_) => `(lang(+))
 
@@ -91,47 +89,13 @@ def unexpsnderMul : Unexpander
 def unexpsnderPow : Unexpander
   | `($_) => `(lang(^))
 
-@[app_unexpander SubTerm.func]
-def unexpandFunc : Unexpander
-  | `($_ $c ![])                 => `(ᵀ“ [$c]() ”)
-  | `($_ $f ![ᵀ“ $t ”])          => `(ᵀ“ [$f]($t) ”)
-  | `($_ $f ![ᵀ“ $t ”, ᵀ“ $u ”]) => `(ᵀ“ [$f]($t, $u) ”)
-  | _                            => throw ()
-
-@[app_unexpander SubTerm.shift]
+@[app_unexpander FunLike.coe]
 def unexpandShift : Unexpander
-  | `($_ ᵀ“$t”) => `(ᵀ“ ᵀ⇑$t ”)
-  | _           => throw ()
-
-@[app_unexpander SubTerm.Hom.toFun]
-def unexpandHom : Unexpander
-  | `($_ shift                   ᵀ“$t”) => `(ᵀ“ ᵀ⇑$t ”)
-  | `($_ bSubst                  ᵀ“$t”) => `(ᵀ“ ⤒$t ”)
-  | `($_ ᵀ⟦→ ![]⟧               ᵀ“$t”) => `(ᵀ“ $t ᵀ⟦⟧ ”)
-  | `($_ ᵀ⟦→ ![ᵀ“$u”]⟧          ᵀ“$t”) => `(ᵀ“ $t ᵀ⟦$u⟧ ”)
-  | `($_ ᵀ⟦→ ![ᵀ“$u₁”, ᵀ“$u₂”]⟧ ᵀ“$t”) => `(ᵀ“ $t ᵀ⟦$u₁, $u₂⟧ ”)
-  | _                                   => throw ()
-
-@[app_unexpander SubTerm.bShift]
-def unexpandBShift : Unexpander
-  | `($_ ᵀ“$t”) => `(ᵀ“ ⤒$t ”)
-  | _           => throw ()
-
-@[app_unexpander SubTerm.substs]
-def unexpandSubsts : Unexpander
-  | `($_ ![]               ᵀ“$t”) => `(ᵀ“ $t ᵀ⟦⟧ ”)
-  | `($_ ![ᵀ“$u”]          ᵀ“$t”) => `(ᵀ“ $t ᵀ⟦$u⟧ ”)
-  | `($_ ![ᵀ“$u₁”, ᵀ“$u₂”] ᵀ“$t”) => `(ᵀ“ $t ᵀ⟦$u₁, $u₂⟧ ”)
-  | _                             => throw ()
-
-@[app_unexpander SubTerm.free]
-def unexpandFree : Unexpander
-  | `($_ ᵀ“$t”) => `(ᵀ“ ᵀᶠ $t ”)
-  | _           => throw ()
-
-@[app_unexpander SubTerm.fix]
-def unexpandFix : Unexpander
-  | `($_ ᵀ“$t”) => `(ᵀ“ ᵀᵇ $t ”)
+  | `($_ ⇑                          ᵀ“$t”) => `(ᵀ“ ᵀ⇑$t ”)
+  | `($_ [→ ]                       ᵀ“$t”) => `(ᵀ“ $t ᵀ[] ”)
+  | `($_ [→ ᵀ“$t₁”]                 ᵀ“$t”) => `(ᵀ“ $t ᵀ[$t₁] ”)
+  | `($_ [→ ᵀ“$t₁”, ᵀ“$t₂”]         ᵀ“$t”) => `(ᵀ“ $t ᵀ[$t₁, $t₂] ”)
+  | `($_ [→ ᵀ“$t₁”, ᵀ“$t₂”, ᵀ“$t₃”] ᵀ“$t”) => `(ᵀ“ $t ᵀ[$t₁, $t₂, $t₃] ”)
   | _           => throw ()
 
 @[app_unexpander SubTerm.func]
@@ -214,7 +178,9 @@ def unexpandFuncArith : Unexpander
 #check (ᵀ“1 + 8” : SubTerm Language.ORingFunc ℕ 8)
 #check (SubTerm.func Language.Mul.mul (ᵀ“1” :> ᵀ“3” :> Matrix.vecEmpty) : SubTerm Language.ORingFunc ℕ 8)
 #check ᵀ“3 + 8 * exp &6 + 2 *#0”
-#check SubTerm.substs ![&0, &5] ᵀ“(3 * #3 + 9)”
+#check [→ &0, &5] ᵀ“3 * #3 + 9”
+#check Rew.shift ᵀ“(3 * #3 + 9)”
+
 end delab
 
 end SubTerm
