Logic/Vorspiel/Vorspiel.lean
@@ -154,6 +154,7 @@ lemma injective_vecCons {f : Fin n → α} (h : Function.Injective f) {a} (ha : 
 
 section And
 
+variable {F : Type _}
 variable [HasLogicSymbols α] [HasLogicSymbols β]
 
 def conj : {n : ℕ} → (Fin n → α) → α
@@ -164,17 +165,18 @@ def conj : {n : ℕ} → (Fin n → α) → α
 
 @[simp] lemma conj_cons {a : α} {v : Fin n → α} : conj (a :> v) = a ⋏ conj v := rfl
 
-@[simp] lemma conj_hom_prop (f : α →L Prop) (v : Fin n → α) : f (conj v) = ∀ i, f (v i) := by
+@[simp] lemma conj_hom_prop [HasLogicSymbols.HomClass F α Prop]
+  (f : F) (v : Fin n → α) : f (conj v) = ∀ i, f (v i) := by
   induction' n with n ih <;> simp[conj]
   · intro ⟨_, _⟩; contradiction
   · simp[ih]; constructor
     · intro ⟨hz, hs⟩ i; cases i using Fin.cases; { exact hz }; { exact hs _ }
     · intro h; exact ⟨h 0, fun i => h _⟩
 
-lemma hom_conj (f : α →L β) (v : Fin n → α) : f (conj v) = conj (f ∘ v) := by
+lemma hom_conj [HasLogicSymbols.HomClass F α β] (f : F) (v : Fin n → α) : f (conj v) = conj (f ∘ v) := by
   induction' n with n ih <;> simp[*, conj]
 
-lemma hom_conj' (f : α →L β) (v : Fin n → α) : f (conj v) = conj fun i => f (v i) := hom_conj f v
+lemma hom_conj' [HasLogicSymbols.HomClass F α β] (f : F) (v : Fin n → α) : f (conj v) = conj fun i => f (v i) := hom_conj f v
 
 end And
 
@@ -376,7 +378,7 @@ def conj : List α → α
 
 @[simp] lemma conj_cons {a : α} {as : List α} : conj (a :: as) = a ⋏ as.conj := rfl
 
-lemma map_conj (f : α →L Prop) (l : List α) : f l.conj ↔ ∀ a ∈ l, f a := by
+lemma map_conj [HasLogicSymbols.HomClass F α Prop] (f : F) (l : List α) : f l.conj ↔ ∀ a ∈ l, f a := by
   induction l <;> simp[*]
 
 def disj : List α → α
@@ -387,7 +389,7 @@ def disj : List α → α
 
 @[simp] lemma disj_cons {a : α} {as : List α} : disj (a :: as) = a ⋎ as.disj := rfl
 
-lemma map_disj (f : α →L Prop) (l : List α) : f l.disj ↔ ∃ a ∈ l, f a := by
+lemma map_disj [HasLogicSymbols.HomClass F α Prop] (f : F) (l : List α) : f l.disj ↔ ∃ a ∈ l, f a := by
   induction l <;> simp[*]
 
 end
@@ -438,12 +440,12 @@ variable [HasLogicSymbols α]
 
 noncomputable def conj (s : Finset α) : α := s.toList.conj
 
-lemma map_conj (f : α →L Prop) (s : Finset α) : f s.conj ↔ ∀ a ∈ s, f a := by
+lemma map_conj [HasLogicSymbols.HomClass F α Prop] (f : F) (s : Finset α) : f s.conj ↔ ∀ a ∈ s, f a := by
   simpa using List.map_conj f s.toList
   
 noncomputable def disj (s : Finset α) : α := s.toList.disj
 
-lemma map_disj (f : α →L Prop) (s : Finset α) : f s.disj ↔ ∃ a ∈ s, f a := by
+lemma map_disj [HasLogicSymbols.HomClass F α Prop] (f : F) (s : Finset α) : f s.disj ↔ ∃ a ∈ s, f a := by
   simpa using List.map_disj f s.toList
 
 end
